Veir/Interpreter/WellFormed.lean
@@ -1,0 +1,183 @@
+import Veir.Interpreter.Basic
+
+namespace Veir
+
+variable {OpInfo : Type} [HasOpInfo OpInfo]
+
+/--
+  A proposition that states that the interpreter state has the execution of a given operation.
+  This means that all the operand and result variables are in the interpreter state, and
+  that the result values are correctly computed from the operand values according to the
+  semantics of the operation.
+-/
+def InterpreterState.SatisfiesEquationLemma (state : InterpreterState) (ctx : IRContext OpCode)
+    (op : OperationPtr) : Prop :=
+  ∃ controlFlow, interpretOp ctx op state = some (state, controlFlow)
+
+/--
+  A well-formedness condition for the interpreter state. It states that every operation
+  result that is in the state has been computed according to the semantics of its defining
+  operation.
+-/
+def InterpreterState.WellFormed (state : InterpreterState) (ctx : IRContext OpCode) : Prop :=
+  ∀ (opRes : OpResultPtr) (opResInBounds : opRes.InBounds ctx),
+  ∀ val, state.getVar? opRes = some val →
+  state.SatisfiesEquationLemma ctx (opRes.get! ctx).owner
+
+@[grind =]
+theorem InterpreterState.getVar?_setVar :
+    (InterpreterState.setVar state var' val).getVar? var =
+    if var = var' then some val else state.getVar? var := by
+  grind [InterpreterState.setVar, InterpreterState.getVar?]
+
+theorem InterpreterState.getVar?_setResultValues_loop
+    {state : InterpreterState} {ctx : IRContext OpInfo} {op} {resultValues} {value}:
+    (state.setResultValues_loop ctx op resultValues idx).getVar? value =
+    match value with
+    | .opResult {op := op', index := index} =>
+      if op' = op ∧ index < idx then
+        some resultValues[index]!
+       else
+         state.getVar? value
+    | _ =>
+      state.getVar? value := by
+  induction idx generalizing state
+  case zero => grind [InterpreterState.setResultValues_loop]
+  case succ idx ih =>
+    simp only [InterpreterState.setResultValues_loop, ih]
+    grind [cases OpResultPtr, OperationPtr.getResult, cases ValuePtr]
+
+@[grind =]
+theorem InterpreterState.getVar?_setResultValues
+    {ctx : IRContext OpInfo} {state : InterpreterState} {op} {resultValues}
+    {value} (valueInBounds : value.InBounds ctx) :
+    (state.setResultValues ctx op resultValues).getVar? value =
+    match value with
+    | .opResult {op := op', index := index} =>
+      if op' = op then
+        some resultValues[index]!
+       else
+         state.getVar? value
+    | _ =>
+      state.getVar? value := by
+  simp only [InterpreterState.setResultValues, InterpreterState.getVar?_setResultValues_loop]
+  cases value
+  next opRes =>
+    by_cases opRes.op = op <;> grind
+  next =>
+    grind
+
+theorem InterpreterState.getVar?_of_interpretOp
+    {state : InterpreterState} {op}
+    (valueInBounds : value.InBounds ctx) :
+    interpretOp ctx op state = some (state', controlFlow) →
+    state'.getVar? value =
+    match value with
+    | .opResult {op := op', index := index} => do
+      if op' = op then
+        let operands := (state.getOperandValues ctx op).get!
+        let opType := op.getOpType! ctx
+        let (resultValues, _) ← interpretOp' opType (op.getProperties! ctx opType) ((op.get! ctx).results.map (·.type)) operands
+        some resultValues[index]!
+       else
+         state.getVar? value
+    | _ =>
+      state.getVar? value := by
+  intro h
+  simp only [interpretOp, Option.pure_def, Option.bind_eq_bind, Option.bind_eq_some_iff,
+    Option.some.injEq, Prod.mk.injEq] at h
+  have ⟨operandValues, hoperandValues, ⟨resValue, cf⟩, hInterp, hstate', hcf⟩ := h; clear h
+  simp only at hcf
+  subst cf state'
+  simp only [InterpreterState.getVar?_setResultValues valueInBounds]
+  cases value <;> grind
+
+def InterpreterState.getOperandValues_inj {op} {ctx : IRContext OpInfo} {state state' : InterpreterState} :
+    (∀ val, val ∈ op.getOperands! ctx → state.getVar? val = state'.getVar? val) →
+    state.getOperandValues ctx op = state'.getOperandValues ctx op := by
+  intro h
+  simp only [getOperandValues]
+  sorry -- Missing lemam in Lean to talk about `mapM`
+
+def InterpreterState.eq_of_interpOp_of_no_results {state : InterpreterState} {op}
+    (hNoResults : op.getNumResults! ctx = 0) :
+    interpretOp ctx op state = some (state', cf) →
+    state = state' := by
+  simp [interpretOp, setResultValues, hNoResults, setResultValues_loop, Option.bind_eq_some_iff]
+
+/--
+  A proposition that states that the interpreter state has not yet interpreted a given operation.
+-/
+def InterpreterState.NotIntepreted (state : InterpreterState) (ctx : IRContext OpCode)
+    (op : OperationPtr) : Prop :=
+  ∀ idx, idx < op.getNumResults! ctx → state.getVar? (op.getResult idx) = none
+
+theorem InterpreterState.SatisfiesEquationLemma_iff_not_NotIntepreted (state : InterpreterState)
+    (wf : state.WellFormed ctx) (ctxWF : ctx.WellFormed)
+    (op : OperationPtr) (opInBounds : op.InBounds ctx) (hasResults : op.getNumResults! ctx ≠ 0) :
+    state.SatisfiesEquationLemma ctx op ↔ ¬ state.NotIntepreted ctx op := by
+  simp only [InterpreterState.SatisfiesEquationLemma, InterpreterState.NotIntepreted]
+  constructor
+  · rintro ⟨controlFlow, hEqLemma'⟩ hNotInterp
+    have hNotInterp := hNotInterp 0 (by grind)
+    have : (op.getResult 0).InBounds ctx := by grind
+    have hinterp := getVar?_of_interpretOp (value := op.getResult 0) (by grind) hEqLemma'
+    simp only [hNotInterp, OperationPtr.getResult_op, ↓reduceIte, OperationPtr.getResult_index,
+      Option.bind_eq_bind] at hinterp
+    sorry -- Missing lemma about getOperandValues
+  · simp only [Classical.not_forall, forall_exists_index, Option.ne_none_iff_exists]
+    intro idx hidx value hvalue
+    simp only [WellFormed] at wf
+    have hEqLemma := wf (op.getResult idx) (by grind) value (by grind)
+    simp only [InterpreterState.SatisfiesEquationLemma] at hEqLemma
+    grind [IRContext.WellFormed, Operation.WellFormed]
+
+theorem InterpreterState.SatisfiesEquationLemma_or_not_NotIntepreted {state : InterpreterState}
+    (wf : state.WellFormed ctx) (ctxWF : ctx.WellFormed)
+    {op : OperationPtr} (opInBounds : op.InBounds ctx)
+    (hasResults : op.getNumResults! ctx ≠ 0) :
+    state.SatisfiesEquationLemma ctx op ∨ state.NotIntepreted ctx op := by
+  by_cases hEqLemma : state.SatisfiesEquationLemma ctx op
+  · grind
+  · grind [InterpreterState.SatisfiesEquationLemma_iff_not_NotIntepreted]
+
+theorem interpretOp_satisfiesEquationLemma_self
+    {state : InterpreterState} (wf : state.WellFormed ctx) {op}:
+    interpretOp ctx op state = some (state', controlFlow) →
+    state'.SatisfiesEquationLemma ctx op := by
+  sorry -- This needs the fact that an operation result is not one of its operands
+
+theorem interpretOp_satisfiesEquationLemma
+    {state : InterpreterState} (wf : state.WellFormed ctx) (ctxWF : ctx.WellFormed)
+    {op} (opInBounds : op.InBounds ctx) :
+    interpretOp ctx op state = some (state', controlFlow) →
+    state.SatisfiesEquationLemma ctx op' →
+    state'.SatisfiesEquationLemma ctx op' := by
+  intro hInterp hEqLemma
+  by_cases hEq : op = op'
+  · subst op
+    grind [interpretOp_satisfiesEquationLemma_self]
+  · by_cases hNumResults : op.getNumResults! ctx = 0
+    · have := @InterpreterState.eq_of_interpOp_of_no_results
+      grind
+    · cases InterpreterState.SatisfiesEquationLemma_or_not_NotIntepreted wf ctxWF opInBounds hNumResults
+      next hEqLemma' => grind [InterpreterState.SatisfiesEquationLemma]
+      next hNotInterp =>
+        simp [InterpreterState.SatisfiesEquationLemma] at ⊢ hEqLemma
+        have ⟨controlFlow, hEqLemma'⟩ := hEqLemma; clear hEqLemma
+        exists controlFlow
+        simp only [interpretOp, Option.pure_def, Option.bind_eq_bind, Option.bind_eq_some_iff] at ⊢ hEqLemma'
+        have ⟨operandVal, hOperandVal, ⟨resVal, cf⟩, hResVal, hEqLemma⟩ := hEqLemma'; clear hEqLemma'
+        simp only [Option.some.injEq, Prod.mk.injEq] at hEqLemma
+        have ⟨hState, _⟩ := hEqLemma; clear hEqLemma
+        subst cf
+        exists operandVal
+        have : (∀ val, val ∈ op'.getOperands! ctx → state'.getVar? val = state.getVar? val) := by sorry
+        simp only [InterpreterState.getOperandValues_inj this, hOperandVal, Option.some.injEq,
+          Prod.mk.injEq, Prod.exists, exists_eq_right_right, true_and]
+        exists resVal
+        simp only [hResVal, true_and]
+        ext var value
+        rw [InterpreterState.getVar?_setResultValues]
+        · sorry
+        · sorry
